theories/Shallow/Soundness.v
@@ -677,10 +677,8 @@ Module Type Soundness
       - (* stm_match_bvec_split *)
         rewrite wp_demonic_match_bvec_split in HYP.
         apply rule_stm_match_bvec_split. cbn; intros.
-        apply rule_pull; intro Heval. apply IHs.
-        remember (eval e δ1). destruct bv.appView.
-        apply bv.app_inj in Heval.
-        now destruct Heval; subst.
+        apply rule_pull; intro Heval; rewrite Heval, bv.appView_app in HYP.
+        now apply IHs.
 
       - (* stm_read_register *)
         destruct HYP as [v HYP].
